in progress: isim_bind coinduction?

cancellation/Cancel.v
@@ -11,7 +11,7 @@ Require Import Any.
 Require Export STB.
 Require Import HPSim ISim ISimClosed.
 Require Import ModSimFacts.
-Require Import MainAdequacy CtxRefine ClosedAdequacy.
+Require Import MainAdequacy CtxRefine CtxRefineFacts ClosedAdequacy.
 Require Import Events SMod HMod Mod.
 
 Set Implicit Arguments.
@@ -55,12 +55,31 @@ Section INTERP.
 
   Definition prog (ms: HModSem.t) : callE ~> itree hmodE :=
     fun _ '(Call fn args) =>
-      '(_, body) <- (alist_find fn ms.(HModSem.fnsems))!;;
-      body args.
-      (* lbody <- (alist_find fn ms.(HModSem.fnsems))!;; *)
-      (* HModSem.sandbox_body lbody args. *)
-    
+      (* '(_, body) <- (alist_find fn ms.(HModSem.fnsems))!;; *)
+      (* body args. *)
+      lbody <- (alist_find fn ms.(HModSem.fnsems))!;;
+      HModSem.sandbox_body lbody args.
+
+      
+  Definition interp_hpI_fbody (ms: HModSem.t)
+    : (list string * (Any.t -> itree hmodE Any.t)) -> (list string * (Any.t -> itree hmodE Any.t))
+    :=
+    fun '(k, b) => (k, interp_hpI_fun (prog ms) b).
+
+
+  Definition wrap_sandbox scopeS: list string * (Any.t -> itree hmodE Any.t) -> list string * (Any.t -> itree hmodE Any.t)
+    := 
+    fun kb => (scopeS, HModSem.sandbox_body kb).
+
+  Definition wrap_elimI ms: list string * (Any.t -> itree hmodE Any.t) -> list string * (Any.t -> itree hmodE Any.t)
+    :=
+    fun kb => interp_hpI_fbody ms (wrap_sandbox ms.(HModSem.scopes) kb). 
+
+
+
 End INTERP.
+
+
 
 
 Module HIRed.
@@ -68,13 +87,14 @@ Module HIRed.
     Context `{Σ: GRA.t}.
 
     Variable ms: HModSem.t.
-  
-    (* Lemma bisim_iter_handle_bind i k:
+    
+    Lemma bisim_iter_handle_bind i k:
       ITree.iter (handle_callE (prog ms)) (i >>= k)
       ≅
       x <- (ITree.iter (handle_callE (prog ms)) i);; ITree.iter (handle_callE (prog ms)) (k x).
     Proof.
-      ginit. revert i k. gcofix CIH. i.
+      eapply (@gpaco2_init _ _ _ _ (eqitC eq false false)); eauto with paco.
+      revert i k. gcofix CIH. i.
       ides i.
       - grind. rewrite/__ [_ _ (Ret _)]unfold_iter_eq. grind.
         gfinal. right. eapply paco2_mon_bot; eauto.
@@ -94,16 +114,16 @@ Module HIRed.
         }
         destruct s.
         {
-          grind. gstep. econs.
-          eapply eqit_clo_trans; eauto.
+          grind. gstep. econs. 
+          guclo eqit_clo_trans; eauto.
           econs; cycle 1.
           { refl. }
-          { eapply CIH. }
+          { gbase. eapply CIH. }
           { instantiate (1:= eq). i. subst. refl. }
           { i. subst. refl. }
           grind. 
-          replace (` x : X <- prog m c;; (tau;; ITree.subst k (k0 x)))
-          with (` r0 : X <- prog m c;; ` x : Any.t <- (tau;; k0 r0);; k x) by grind.
+          replace (` x : X <- prog ms c;; (tau;; ITree.subst k (k0 x)))
+          with (` r0 : X <- prog ms c;; ` x : Any.t <- (tau;; k0 r0);; k x) by grind.
           refl.
         } 
         destruct s.
@@ -113,7 +133,8 @@ Module HIRed.
         }
         grind. rewrite! bind_trigger. gstep. econs. i.
         r. grind. gstep. econs. gbase. eauto.
-    Qed. *)
+      Unshelve. eauto with paco.
+    Qed.
 
     Lemma iter_handle_bind i k:
       ITree.iter (handle_callE (prog ms)) (i >>= k)
@@ -203,6 +224,140 @@ Module HIRed.
   End RED.
 End HIRed.
 
+Section CANCEL.
+  Context `{Σ: GRA.t}.
+
+  (* Variable md: HMod.t.
+  Variable ginv: Sk.t -> invspec.
+  Variable stb: Sk.t -> gname -> option fspec.
+
+  Let sk: Sk.t := HMod.sk md. *)
+
+  Definition bindRR {R} Ist CIH : nat -> alist key Any.t * R-> alist key Any.t * R -> iProp :=
+    fun nths '(st0, ret0) '(st1, ret1) => ((⌜ret0 = ret1⌝ ∗ Ist nths st0 st1) ∗ □CIH)%I.
+
+  Definition progI fl : callE ~> itree hmodE :=
+    fun _ '(Call fn args) =>
+      lbody <- (alist_find fn fl)!;;
+      lbody args.
+
+  Lemma iter_bind_I fl i k:
+    ITree.iter (handle_callE (progI fl)) (i >>= k)
+    =
+    x <- (ITree.iter (handle_callE (progI fl)) i);; ITree.iter (handle_callE (progI fl)) (k x).
+  Proof. 
+  Admitted.
+
+  Lemma bind_I
+    fl itr ktr
+  :
+    interp_hpI (progI fl) (itr >>= ktr)
+    =
+    x <- interp_hpI (progI fl) itr;; interp_hpI (progI fl) (ktr x).
+  Proof.
+    rewrite/interp_hpI iter_bind_I. refl.
+  Qed.
+
+
+  Lemma cancelI
+      (* prog *)
+      fl my_tid nths
+      ps pt
+      st_src st_tgt (itr: itree hmodE Any.t)
+      (* scopes *)
+      (* + something about function scopes found in fls, flt *)
+    :
+    IstEq0 nths st_src st_tgt
+    ⊢ isim fl fl IstEq0 my_tid true ibot ibot
+       (fun nths '(st_src, v_src) '(st_tgt, v_tgt) => (⌜v_src = v_tgt⌝ ∗ IstEq0 nths st_src st_tgt)%I)
+       ps pt nths (st_src, interp_hpI (progI fl) itr) (st_tgt, itr).
+       (* ps pt nths (st_src, interp_hpI (progI fl) (HModSem.sandbox scopes itr)) (st_tgt, (HModSem.sandbox scopes itr)). *)
+  Proof.
+    revert itr.
+    revert st_tgt. apply combine_quant_dep.
+    revert st_src. apply combine_quant_dep.
+    (* revert scopes. apply combine_quant. *)
+    revert pt. apply combine_quant_dep.
+    revert ps. apply combine_quant_dep.
+    revert nths. apply combine_quant_dep.
+    eapply isim_coind. i.
+
+    destruct a as [nths [ps [pt [st_src [st_tgt it]]]]]. s.
+    (* destruct a as [nths [ps [pt [scopes [st_src [st_tgt it]]]]]]. s. *)
+    iIntros "(#(_ & CIH) & Ist)".
+    
+    assert (CASE := case_itrH _ it); des; subst.
+    - rewrite/__ HIRed.ret. step. eauto.
+    - rewrite/__ HIRed.tau. steps_l. steps_r. by_coind "CIH". eauto.
+    - rewrite/__ HIRed.bind_ag. 
+      steps_l. force_r. iFrame. by_coind "CIH". eauto.
+    - rewrite/__ HIRed.bind_ag. 
+      steps_r. force_l. iFrame. steps_l. by_coind "CIH". eauto.
+    - rewrite/__ HIRed.bind_sch. depdes s.
+      + step. steps_l. by_coind "CIH". auto.
+      + iApply isim_yield. iFrame. iIntros (? ? ? ? ?) "IST".
+        steps_l. by_coind "CIH". auto.
+      + steps_l. steps_r. by_coind "CIH". auto.
+    - destruct c. rewrite/__ HIRed.call. steps_l. 
+
+      destruct (alist_find fn fl) eqn:FIND; cycle 1.
+      { 
+        (* rewrite/__ HModSB.transl_bind HModSB.transl_call. *)
+        iApply isim_call_none; ss.
+        unfold triggerNB. steps_r. ss.
+      }
+      iApply isim_inline_tgt; eauto.
+      s. ired. rewrite/__ bind_I.
+      remember (∀ a : {_ : nat & {_ : bool & {_ : bool & {_ : alist key Any.t & {_ : alist key Any.t & itree hmodE Any.t}}}}},
+      IstEq0 (projT1 a) (projT1 (projT2 (projT2 (projT2 a)))) (projT1 (projT2 (projT2 (projT2 (projT2 a))))) -∗
+      g0 Any.t (λ (nths0 : nat) '(st_src0, v_src) '(st_tgt0, v_tgt), ⌜v_src = v_tgt⌝ ∗ IstEq0 nths0 st_src0 st_tgt0)
+        (projT1 (projT2 a)) (projT1 (projT2 (projT2 a))) (projT1 a)
+        (projT1 (projT2 (projT2 (projT2 a))), interp_hpI (progI fl) (projT2 (projT2 (projT2 (projT2 (projT2 a))))))
+        (projT1 (projT2 (projT2 (projT2 (projT2 a)))), projT2 (projT2 (projT2 (projT2 (projT2 a))))))%I.
+      iApply isim_bind; cycle 1.
+      {
+        instantiate (1:= (fun nths '(st_src, v_src) '(st_tgt, v_tgt) => (⌜v_src = v_tgt⌝ ∗ IstEq0 nths st_src st_tgt ∗ □b)%I)).
+        (* by_coind "CIH". eauto.   *)
+
+        (* Check (@bindRR Any.t IstEq0 b).  *)
+        rewrite Heqb.
+        (* instantiate (1:= @bindRR Any.t IstEq0 b).  *)
+        iApply isim_progress; iApply isim_base.
+        iSpecialize ("CIH" $! _); repeat instantiate (1:= existT _ _); s.
+        (* unfold bindRR. *)
+        (* iApply "CIH". *)
+        (* instantiate (1:= EqRR ). *)
+        (* by_coind "CIH".   *)
+        (* admit. *)
+        admit.
+      }
+      i. iIntros "(% & IST & #CIH)". des. subst.
+      rewrite HIRed.tau. steps_l. steps_r. ired.
+      by_coind "CIH". auto.
+    - iDestruct "Ist" as "%". depdes s.
+      + rewrite/__ HIRed.bind_pg. iApply isim_sput_src. iApply isim_sput_tgt. steps_l.
+        by_coind "CIH". iPureIntro. subst. eauto.
+      + rewrite/__ HIRed.bind_pg. iApply isim_sget_src. iApply isim_sget_tgt. steps_l.
+        subst. unfold or_else. des_ifs; by_coind "CIH"; eauto.
+    - rewrite HIRed.bind_core. depdes e.
+      + steps_r. force_l. steps_l.
+        instantiate (1:= q). by_coind "CIH". eauto.
+      + steps_l. force_r. instantiate (1:= q).
+        by_coind "CIH". auto.
+      + step. steps_l. by_coind "CIH". auto.
+    Unshelve. all: eauto.
+  Admitted.
+
+
+
+   (* Ist nths st_src st_tgt ⊢ *)
+     (* @isim Σ fl_src fl_tgt Ist my_tid is_closed ibot ibot Any.t *)
+     (* (fun nths '(st_src, v_src) '(st_tgt, v_tgt) => (⌜v_src = v_tgt⌝ ∗ Ist nths st_src st_tgt))%I *)
+     (* false false nths (st_src, itr_src) (st_tgt, itr_tgt)))%signature. *)
+    
+End CANCEL.
+
+
 (* elimI: call-inlined HMod. *)
 (* elimIC: inlined & cancelled *)
 (* elimC : call remaining, cancelled *)
@@ -213,15 +368,17 @@ Module HModSemAux.
 
     Program Definition to_elimI (ms: HModSem.t): HModSem.t := {|
       HModSem.scopes := ms.(scopes);
-      HModSem.fnsems := List.map (map_snd (λ ksb, (ksb.1, interp_hpI_fun (prog ms) ksb.2))) (ms.(fnsems));
+      HModSem.fnsems := List.map (map_snd (wrap_elimI ms)) (ms.(fnsems));
+      (* HModSem.fnsems := List.map (map_snd (λ ksb, (ksb.1, interp_hpI_fun (prog ms) ksb.2))) (ms.(fnsems)); *)
       HModSem.initial_st := ms.(initial_st);
     |}.
     Next Obligation.
       i. depdes ms. ss. ii. unfold fnsems_scopes in *. unfold map_snd in*.
       rewrite! alist_find_map in H. unfold o_map in H.
-      des_ifs; ss. inv Heq0.
+      des_ifs; ss. 
+      (* inv Heq0.
       specialize (well_scoped_fns0 fn a).
-      des_ifs; ss. inv Heq. eauto.
+      des_ifs; ss. inv Heq. eauto. *)
     Qed.
     Next Obligation. ii. destruct ms. ss. eauto. Qed.
     Next Obligation. ii. destruct ms. ss. eauto. Qed.
@@ -265,55 +422,55 @@ Section CANCEL.
 ) *)
 
   Lemma alist_find_elimI
-      ms fn fs scopes
-      (FINDS: alist_find fn (HModSem.fnsems (HModSemAux.to_elimI ms)) = Some (scopes, fs))
+      ms fn fs
+      (FINDS: alist_find fn (HModSem.fnsems (HModSemAux.to_elimI ms)) = Some fs)
     :
-    exists ft, fs = interp_hpI_fun (prog ms) ft.
+    exists ft, 
+      fs = interp_hpI_fbody ms (wrap_sandbox (ms.(HModSem.scopes)) ft) /\
+      incl ft.1 ms.(HModSem.scopes)
+      .
   Proof.
   Admitted. 
 
-
-  Definition bindRR {R} Ist CIH : nat -> alist key Any.t * R-> alist key Any.t * R -> iProp :=
-    fun nths '(st0, ret0) '(st1, ret1) => ((⌜ret0 = ret1⌝ ∗ Ist nths st0 st1) ∗ □CIH)%I.
+  (* Definition bindRR {R} Ist CIH : nat -> alist key Any.t * R-> alist key Any.t * R -> iProp := *)
+    (* fun nths '(st0, ret0) '(st1, ret1) => ((⌜ret0 = ret1⌝ ∗ Ist nths st0 st1) ∗ □CIH)%I. *)
 
     (* (⌜v_src = v_tgt⌝ ∗ Ist nths st_src st_tgt))%I *)
 
 
-  Lemma cancel0 IC
-    scopes fs ft
+
+  Lemma cancel0
+    (* scopes fs ft
     (MAIN: 
       ∀sk0 (SKINCL: incl (HMod.sk md) sk0) (SKWF: Sk.wf sk0),
         (alist_find "CRIS_main" (HModSem.fnsems (HModSemAux.to_elimI (HMod.modsem md sk0)))
           = Some (scopes, fs)) /\
         (alist_find "CRIS_main" (HModSem.fnsems (HMod.modsem md sk0))
           = Some (scopes, ft)) /\
-        (fs = interp_hpI_fun (prog (HMod.modsem md sk0)) ft))
+        (fs = interp_hpI_fun (prog (HMod.modsem md sk0)) ft)) *)
   :
-    HSimC.t (HModAux.to_elimI md) md IC IstEq.
+    (* HSimC.t (HModAux.to_elimI md) md IC IstEq. *)
+    refines (HModAux.to_elimI md, const(emp%I)) (md, const(emp%I)).
   Proof.
+    eapply closed_adequacy.
+    instantiate (1:= IstEq).
     econs; ss. i. r.
     econs; ss; try refl.
     { iIntros "_". iPureIntro. ss. }
     { rewrite map_length. ss. }
     { i. rewrite/__ map_map_compose fst_map_snd in IN. ss. }
-    specialize (MAIN sk0 SKINCL SKWF). des.
-    econs. esplits; eauto.
-    assert ((scopes, fs) = fs0).
-    { rewrite/HModSemAux.to_elimI MAIN in FIND. inv FIND. ss. }
-    subst fs0. 
-    ii. subst.
-    (* iIntros "%". subst. *)
+    ii. hexploit FIND. i. destruct fs.
+    eapply alist_find_elimI in H. des. exists ft.
+    esplits. { admit. }
+    ii. subst. destruct ft. s in H0.
+    unfold wrap_sandbox, interp_hpI_fbody in H. s in H.
+    inv H. revert H0.
+    generalize (HModSem.scopes (HMod.modsem md sk0)) as scopeS. i.
+    rename l0 into scopeT. rename H0 into INCL.
     unfold HModSem.sandbox_body, interp_hpI_fun. s.
-    (* unfold HModSem.sandbox at 3 4. *)
-    (* iIntros "%". subst. iStopProof. *)
-
-    generalize scopes at 1. intros scopesS.
-    generalize scopes. intros scopesT.
-    (* Should be scopesT ⊆ scopesS *)
-
-    generalize (ft y) as it. clear MAIN MAIN0 FIND ft y.
     generalize false at 1 as ps.
     generalize false at 1 as pt. intros pt ps.
+    generalize (i0 y) as it. clear IN fn FIND i0 y.
 
     (* remember (λ (nths0 : nat) '(st_src, v_src) '(st_tgt0, v_tgt), ⌜v_src = v_tgt⌝ ∗ *)
     (* IstEq sk0 nths0 st_src st_tgt0)%I as RR. *)
@@ -321,15 +478,16 @@ Section CANCEL.
     revert NODS. apply combine_quant.
     revert st_tgt. apply combine_quant_dep.
     revert st_src. apply combine_quant_dep.
-    revert scopesT. apply combine_quant.
-    revert scopesS. apply combine_quant_dep.
+    revert INCL. apply combine_quant.
+    revert scopeT. apply combine_quant_dep.
+    revert scopeS. apply combine_quant_dep.
     (* revert HeqRR. apply combine_quant_dep. *)
     (* revert RR. apply combine_quant_dep. *)
 
 
     (* revert st_src. apply combine_quant_dep. *)
-    revert pt. apply combine_quant_dep.
-    revert ps. apply combine_quant_dep.
+    revert pt. apply combine_quant.
+    revert ps. apply combine_quant.
     revert nths. apply combine_quant.
     eapply isim_coind. i.
 
@@ -362,13 +520,13 @@ Section CANCEL.
 
     (* rewrite Heqb. *)
 
-    destruct a as [nths [ps [pt [scopeS [scopeT [st_src [st_tgt [NODS [NODD it]]]]]]]]]. s.
+    destruct a as [nths [ps [pt [scopeS [scopeT [INCL [st_src [st_tgt [NODS [NODD it]]]]]]]]]]. s.
     iIntros "(#(_ & CIH) & Ist)".
     
     
     assert (CASE := case_itrH _ it); des; subst.
-    - rewrite HIRed.ret. step. eauto.
-    - rewrite HIRed.tau. steps_l. steps_r. by_coind "CIH". eauto.
+    - rewrite/__ HModSB.transl_ret HIRed.ret. step. eauto.
+    - rewrite/__ HModSB.transl_tau HIRed.tau. steps_l. steps_r. by_coind "CIH". eauto.
     - rewrite HIRed.bind_ag. steps_l. force_r. iFrame. by_coind "CIH". eauto.
     - rewrite HIRed.bind_ag. steps_r. force_l. iFrame. steps_l. by_coind "CIH". eauto.
     - rewrite HIRed.bind_sch. depdes s.
@@ -402,24 +560,16 @@ Section CANCEL.
       rewrite HIRed.tau. steps_l. steps_r. ired.
       (* by_coind "CIH". auto. *)
       admit.
-    - admit.
+    - depdes s.
+      + rewrite/__ HIRed.bind_pg !HModSB.transl_bind !HModSB.transl_put. 
+    
+    
+    admit.
     - rewrite HIRed.bind_core. depdes e.
       + steps_r. force_l. steps_l.
         instantiate (1:= q). by_coind "CIH". eauto.
       + steps_l. force_r. instantiate (1:= q).
         by_coind "CIH". auto.
       + step. steps_l. by_coind "CIH". auto.
-    
-
-
-
-    assert (FINDT:= alist_find_elimI).
-    specialize (FINDT _ _ _ _ FIND). des.
-    esplits. 
-    { instantiate (1:= (l, ft)). }
-
-    
-
-
 
 End CANCEL.
